NFormula.thy
@@ -1,0 +1,78 @@
+theory NFormula
+imports Small_Step
+begin
+
+type_synonym assn = "newstate \<Rightarrow> bool"
+
+type_synonym active_addrs = "nat \<Rightarrow> bool"
+
+definition dom::"active_addrs \<Rightarrow> nat set" where "dom bs \<equiv> {addr. bs addr}"
+
+datatype formula = Bc bool | 
+  Not formula| 
+  And formula formula|
+  Or formula formula| 
+  Less aexp aexp|
+  Greater aexp aexp|
+  Equal aexp aexp|
+  Imp formula formula|
+  Forall vname formula| 
+  Exist vname formula|
+  Points_to aexp aexp ("_ \<mapsto> _")|
+  Conj formula formula ("_ * _")
+
+fun extFree::"aexp \<Rightarrow> vname list" where
+"extFree (N n) = []"|
+"extFree (V v) = [v]"|
+"extFree (Plus a1 a2) = (extFree a1) @ (extFree a2)"
+
+fun extractFree::"formula \<Rightarrow> vname list" where
+"extractFree (Bc v) = []"|
+"extractFree (Not f) = (extractFree f)"|
+"extractFree (And f1 f2) = (extractFree f1) @ (extractFree f2)"|
+"extractFree (Or f1 f2) = (extractFree f1) @ (extractFree f2)"|
+"extractFree (Less a1 a2) = ((extFree a1) @ (extFree a2))"|
+"extractFree (Greater a1 a2) = ((extFree a1) @ (extFree a2))"|
+"extractFree (Equal a1 a2) = ((extFree a1) @ (extFree a2))"|
+"extractFree (Imp f1 f2) = (extractFree f1) @ (extractFree f2)"|
+"extractFree (Forall v f) = (removeAll v (extractFree f))"|
+"extractFree (Exist v f) = (removeAll v (extractFree f))"|
+"extractFree (Points_to a1 a2) = ((extFree a1) @ (extFree a2))"|
+"extractFree (Conj f1 f2) = (extractFree f1) @ (extractFree f2)"
+
+value "extractFree(Or (Forall ''y'' (Less (V ''y'') (V ''z''))) (Less (V ''y'') (V ''x'')))"
+value "extractFree(Or (Forall y (Less (V y) (V z))) (Less (V y) (V x)))"
+
+fun getAddr::"formula \<Rightarrow> newstate \<Rightarrow> nat set" where
+"getAddr (Bc v) s = {}"|
+"getAddr (Not f) s = (getAddr f s)"|
+"getAddr (And f1 f2) s = (getAddr f1 s) \<union> (getAddr f2 s)"|
+"getAddr (Or f1 f2) s = (getAddr f1 s) \<union> (getAddr f2 s)"|
+"getAddr (Less a1 a2) s = {}"|
+"getAddr (Greater a1 a2) s = {}"|
+"getAddr (Equal a1 a2) s = {}"|
+"getAddr (Imp f1 f2) s = (getAddr f1 s) \<union> (getAddr f2 s)"|
+"getAddr (Forall v f) s = (getAddr f s)"|
+"getAddr (Exist v f) s = (getAddr f s)"|
+"getAddr (Points_to a1 a2) s = {addr. addr = aval a1 (vars s)}"|
+"getAddr (Conj f1 f2) s = (getAddr f1 s) \<union> (getAddr f2 s)"
+
+fun fVal::"formula \<Rightarrow> active_addrs \<Rightarrow> newstate \<Rightarrow> bool" where
+"fVal (Bc v) bs s = v"|
+"fVal (Not f) bs s = (\<not>fVal f bs s)"|
+"fVal (And f1 f2) bs s = ((fVal f1 bs s) \<and> (fVal f2 bs s))"|
+"fVal (Or f1 f2) bs s = ((fVal f1 bs s) \<or> (fVal f2 bs s))"|
+"fVal (Less a1 a2) bs s = ((aval a1 (vars s)) < (aval a2 (vars s)))"|
+"fVal (Greater a1 a2) bs s = ((aval a1 (vars s)) > (aval a2 (vars s)))"|
+"fVal (Equal a1 a2) bs s = ((aval a1 (vars s)) = (aval a2 (vars s)))"|
+"fVal (Imp f1 f2) bs s = ((fVal f1 bs s) \<longrightarrow> (fVal f2 bs s))"|
+"fVal (Forall v f) bs s = (fVal f bs s)"|
+"fVal (Exist v f) bs s = (fVal f bs s)"|
+"fVal (Points_to a1 a2) bs s = (((mem s)(aval a1 (vars s)) = (aval a2 (vars s))) \<and> bs (aval a1 (vars s)))"|
+"fVal (Conj f1 f2) bs s = ((getAddr f1 s) \<inter> (getAddr f2 s) = {} \<and> 
+  (\<forall>addr \<in> (getAddr f1 s). (bs addr)) \<and> (\<forall>addr \<in> (getAddr f2 s). (bs addr)) \<and> (fVal f1 bs s) \<and> (fVal f2 bs s))"
+
+definition condition :: "formula \<Rightarrow> com \<Rightarrow> bool"
+  where "condition f c \<equiv> \<forall> bs s s' . fVal f bs s \<and> (Some c, s) \<Rightarrow>\<^sub>t\<^sub>r s' \<longrightarrow> fVal f bs s'"
+
+end
